expect return expected element

test/Token.v
@@ -1,15 +1,23 @@
 From Parsec Require Export
      Core.
 
-(* https://httpwg.org/http-core/draft-ietf-httpbis-semantics-latest.html#rule.token.separators *)
+(** https://httpwg.org/http-core/draft-ietf-httpbis-semantics-latest.html#rule.token.separators *)
 
 Definition istchar (a : ascii) : bool :=
-  isalpha a || isdigit a || in_string "!#$%&'*+-.^_`|~" a.
+  isalpha a ||| isdigit a ||| in_string "!#$%&'*+-.^_`|~" a.
 
 Definition parseToken : parser string :=
   string_of_list_ascii <$> many1 (satisfy istchar).
 
 Goal parse parseToken "GET / HTTP/1.1" = inr "GET".
+Proof. reflexivity. Qed.
+
+(** https://www.rfc-editor.org/rfc/rfc3986.html#section-2.1 *)
+Definition parsePctEncoded : parser string :=
+  liftA2 String (expect "%"%char)
+         (string_of_list_ascii <$> manyN 2 (satisfy ishexdig)).
+
+Goal parse parsePctEncoded "%123" = inr "%12".
 Proof. reflexivity. Qed.
 
 Goal string_of_list_ascii <$>
