theories/Core.v
@@ -4,19 +4,19 @@ From Parsec Require Export
 (** https://www.rfc-editor.org/rfc/rfc5234.html#appendix-B.1 *)
 
 Definition isbit : ascii -> bool := in_string "01".
-Definition isalpha (a : ascii) : bool := isupper a || islower a.
-Definition ischar  (a : ascii) : bool := (("001" <=? a) && (a <=? "127"))%char.
-Definition isctl   (a : ascii) : bool := ((a <=? "031") || (a =? "127"))%char.
+Definition isalpha (a : ascii) : bool := isupper a ||| islower a.
+Definition ischar  (a : ascii) : bool := (("001" <=? a) &&& (a <=? "127"))%char.
+Definition isctl   (a : ascii) : bool := ((a <=? "031") ||| (a =? "127"))%char.
 
-Definition parseHTAB   : parser unit := expect "009"%char.
-Definition parseLF     : parser unit := expect "010"%char.
-Definition parseCR     : parser unit := expect "013"%char.
-Definition parseSP     : parser unit := expect " "%char.
-Definition parseDQUOTE : parser unit := expect """"%char.
+Definition parseHTAB   : parser ascii := expect "009"%char.
+Definition parseLF     : parser ascii := expect "010"%char.
+Definition parseCR     : parser ascii := expect "013"%char.
+Definition parseSP     : parser ascii := expect " "%char.
+Definition parseDQUOTE : parser ascii := expect """"%char.
 
 Open Scope parser_scope.
 
-Definition parseCRLF : parser unit := parseCR;; parseLF.
-Definition parseWSP  : parser unit := parseSP <|> parseHTAB.
+Definition parseCRLF : parser unit := parseCR;; parseLF;; ret tt.
+Definition parseWSP  : parser ascii := parseSP <|> parseHTAB.
 Definition parseLWSP : parser unit :=
   many (parseWSP <|> (parseCRLF ;; parseWSP));; ret tt.
